Move to new automaton module.

src/dafny/utils/Automata.dfy
@@ -13,7 +13,8 @@
  */
 
 include "./MiscTypes.dfy"
-include "./Partition.dfy"
+include "../utils/int.dfy"
+include "../utils/LinSegments.dfy"
 
 /** 
   * Provides finite automata.
@@ -21,37 +22,183 @@ include "./Partition.dfy"
 module Automata {
 
   import opened MiscTypes
-  import opened PartitionMod
+  import opened Int
+  import opened LinSegments
 
-  type ValidAuto = a: Auto | a.IsValid() witness Auto(0, map[])
+  /** A valid automaton satisfies some invariants given by IsValid(). */
+  type ValidAuto<!T(!new)> = a: Auto<T> | a.IsValid() witness Auto()
 
-  datatype Auto = Auto(numStates: nat, transitions: map<(nat, bool), nat>)
+  /**
+    *  Automaton.
+    *  @param transitions       The transition function.
+    *  @param transitionsNat    The transition function using the id of the states.
+    *  @param states            The set of states.
+    *  @toString                The string representation of a state.
+    *  @indexOf                 The index of a state.
+    *  @note                    A valid automaton is such that every state has an entry in the transitions map.
+    *                           If the state has no successor then the entry is the empty list.
+    *  @note                    The transition function is givem as transitionsNat, but the datatype
+    *                           uses transitions which is a map from stateId to stateIds. The reason
+    *                           is that it is easier to manipulate the transitions using the stateId .e.g.
+    *                           when minising an automaton.
+    */
+  datatype Auto<!T(!new,==)> =
+    Auto(ghost transitions: map<T, seq<T>> := map[],
+         transitionsNat: map<nat, seq<nat>> := map[],
+         states: seq<T> := [],
+         toString: T -> string := (_  => ""),
+         indexOf: map<T, nat> := map[])
   {
-
-    /** 
-      * The transition function should return states within the numStates range.
-      * Note that the map can have keys (k, l) with states k >= numStates, that's
-      * perfectly accpetable.
-      */
-    predicate IsValid()
+    predicate Equals(b: Auto<T>)
     {
-      forall k:: k in transitions ==> transitions[k] < numStates
+      && transitionsNat == b.transitionsNat
+      && states == b.states
     }
 
     /**
-      *  Successor state of s via l.
-      *  @param  s   A state index.
-      *  @param  l   A label index.
-      *  @returns    The successor of s via l if exists of None otherwise.      
+      * Add a state to the automaton.
+      * @param i  The state to add.
       */
-    function Succ(s: nat, l: bool): Option<nat>
-      requires this.IsValid()
-      requires 0 <= s < numStates
-      ensures Succ(s, l).Some? ==> 0 <= Succ(s, l).v < numStates
+    function {:timeLimitMultiplier 8} AddState(i: T): (a: Auto<T>)
+      requires IsValid()
+      ensures i in a.states
+      ensures a.IsValid()
     {
-      if (s, l) in transitions then Some(transitions[(s, l)])
-      else None
+      if i in states then
+        this
+      else
+        assert (indexOf + map[i := |states|]).Values == indexOf.Values + { |states| };
+        this
+        .(states := states + [i])
+        .(indexOf := indexOf + map[i := |states|])
+        .(transitions := transitions + map[i := []])
+        .(transitionsNat := transitionsNat + map[|states| := []])
+    }
+
+    /**
+      * Add a transition from i to j to the automaton.
+      * @param i  The source state.
+      * @param j  The destination state.
+      * @returns  An automaton with the transition added.  
+      * @note     If i or j are not in the automaton then they are added.
+      * @note     The transitions from i to j are in a seq, and j is added at the end of the seq.
+      */
+    function {:timeLimitMultiplier 8} AddEdge(i: T, j: T): (a: Auto<T>)
+      requires IsValid()
+      ensures a.IsValid()
+    {
+      var a1 := this.AddState(i).AddState(j);
+      if a1.indexOf[j] in a1.transitionsNat[a1.indexOf[i]] then
+        a1
+      else
+        a1
+        .(transitions := a1.transitions + map[i := a1.transitions[i] + [j]])
+        .(transitionsNat := a1.transitionsNat + map[a1.indexOf[i] := a1.transitionsNat[a1.indexOf[i]] + [a1.indexOf[j]]])
+    }
+
+    /**
+      *  Add several transitions from i to all the elements of js.
+      */
+    function AddEdges(i: T, js: seq<T>): (a: Auto<T>)
+      requires IsValid()
+      ensures a.IsValid()
+      decreases |js|
+    {
+      if |js| == 0 then this
+      else this.AddEdge(i, js[0]).AddEdges(i, js[1..])
+    }
+
+    /**
+      * Returns the number of states of the automaton.
+      */
+    function SSize(): nat
+      requires this.IsValid()
+    {
+      |states|
+    }
+
+    function TSize(index: nat := 0): nat
+      requires this.IsValid()
+      requires index <= |states|
+      decreases |states| - index
+    {
+      if index == |states| then 0
+      else
+        |transitionsNat[index]| + TSize(index + 1)
+    }
+
+    /** 
+      *  Successors of a state.
+      *  @param s  The state.
+      *  @returns  The successors of s.
+      */
+    function Succ(s: T): (r: seq<T>)
+      requires this.IsValid()
+      requires s in states
+      ensures r == transitions[s]
+    {
+      seq(|transitionsNat[indexOf[s]]|, i requires 0 <= i < |transitionsNat[indexOf[s]]| => states[transitionsNat[indexOf[s]][i]])
+    }
+
+    /**
+      *  The successors using the id of the states.
+      *  @param      i  The id of the source state.
+      *  @returns        The ids of the successors.
+      */
+    function SuccNat(i: nat): (r: seq<nat>)
+      requires this.IsValid()
+      requires i < |states|
+      ensures forall j: nat :: 0 <= j < |r| ==> r[j] < |states|
+    {
+      transitionsNat[i]
+    }
+
+    /**
+      * String representation of a state.
+      */
+    function ToString(t: T): string {
+      toString(t)
+    }
+
+    /** Print to Dot format. */
+    method {:print} ToDot()
+      requires this.IsValid()
+    {
+      print "digraph G {\n";
+      print "// Number of states: ", NatToString(SSize()), "\n";
+      print "// Number of transitions : ", NatToString(TSize()), "\n";
+      for i := 0 to |states|
+      {
+        print "s_", i, " [label=", ToString(states[i]) + "]\n";
+      }
+      for i := 0 to |states| {
+        for j := 0 to |transitionsNat[i]| {
+          print "s_", i, " -> ", "s_", transitionsNat[i][j],
+                " [label=\"" + NatToString(j) + "\"]"
+                + ";\n";
+        }
+      }
+      print "}\n";
+    }
+
+    /**
+      * Check if the automaton is valid.
+      */
+    ghost predicate IsValid() {
+      && (forall i : T :: i in states <==> i in transitions)
+      && (forall k, k':: 0 <= k < k' < |states| ==> states[k] != states[k'])
+      && (forall i, j :: i in states && 0 <= j < |transitions[i]| ==> transitions[i][j] in states)
+      && (forall s:: s in states <==> s in indexOf)
+      && (forall i:: i in indexOf ==> indexOf[i] < |states| && states[indexOf[i]] == i)
+      && (forall i:: 0 <= i < |states| ==> states[i] in indexOf && indexOf[states[i]] == i)
+      && (indexOf.Values == set z {:nowarn} | 0 <= z < |states|)
+      && (transitionsNat.Keys == set z {:nowarn} | 0 <= z < |states|)
+      && (indexOf.Values == transitionsNat.Keys)
+      && (forall k:: k in transitionsNat ==> |transitionsNat[k]| == |transitions[states[k]]|)
+      && (forall k:: k in transitions ==> |transitions[k]| == |transitionsNat[indexOf[k]]|)
+      && (forall i, j :: 0 <= i < |states| && 0 <= j < |transitionsNat[i]| ==> 0 <= transitionsNat[i][j] < |states|)
+      && ((forall i, j :: 0 <= i < |states| && 0 <= j < |transitionsNat[i]| ==> states[transitionsNat[i][j]] == transitions[states[i]][j]))
+      && ((forall i:T , j :: i in states && 0 <= j < |transitions[i]| ==> indexOf[transitions[i][j]] == indexOf[transitions[i][j]]))
     }
   }
-
 }
